SEQUENCE serialiezr and experiments about proving things over it.

src/asn1/ASN1.Base.fst
@@ -15,8 +15,6 @@ type asn1_type: Type =
 // | OID
 | SEQUENCE
 
-// let asn1_primitive_type = a: asn1_type{a <> SEQUENCE}
-
 let the_asn1_type (a: asn1_type)
 : Tot Type
 = (a': asn1_type{a == a'})
@@ -30,11 +28,7 @@ let asn1_length_max: n: asn1_length_t {forall (n':asn1_length_t). n >= n'} = 429
 let asn1_length_inbound (x: nat) (min max: asn1_length_t): bool
 = min <= x && x <= max
 
-let asn1_int32 = LowParse.Spec.BoundedInt.bounded_int32 asn1_length_min asn1_length_max
-let asn1_int32_min: i: asn1_int32 {forall (i': asn1_int32). i <= i'} = 0ul
-let asn1_int32_max: i: asn1_int32 {forall (i': asn1_int32). i >= i'} = 4294967295ul
-
-let min_of_asn1_type
+let asn1_length_min_of_type
   (a: asn1_type)
 : asn1_length_t
 = match a with
@@ -43,7 +37,7 @@ let min_of_asn1_type
   | OCTET_STRING -> asn1_length_min
   | SEQUENCE -> asn1_length_min
 
-let max_of_asn1_type
+let asn1_length_max_of_type
   (a: asn1_type)
 : asn1_length_t
 = match a with
@@ -52,33 +46,73 @@ let max_of_asn1_type
   | OCTET_STRING -> asn1_length_max
   | SEQUENCE -> asn1_length_max
 
-let bound_of_asn1_type
+let asn1_length_bound_of_type
   (a: asn1_type)
 : (asn1_length_t & asn1_length_t)
-= (min_of_asn1_type a, max_of_asn1_type a)
+= (asn1_length_min_of_type a, asn1_length_max_of_type a)
 
-let asn1_int32_of_tag
+let asn1_length_inbound_of_type
+  (a: asn1_type) (x: nat)
+: bool
+= let min, max = asn1_length_bound_of_type a in
+  asn1_length_inbound x min max
+
+let asn1_int32 = LowParse.Spec.BoundedInt.bounded_int32 asn1_length_min asn1_length_max
+let asn1_int32_min: i: asn1_int32 {forall (i': asn1_int32). i <= i'} = 0ul
+let asn1_int32_max: i: asn1_int32 {forall (i': asn1_int32). i >= i'} = 4294967295ul
+
+let asn1_int32_of_type
   (_a: asn1_type)
-= let min, max = min_of_asn1_type _a, max_of_asn1_type _a in
+= let min, max = asn1_length_min_of_type _a, asn1_length_max_of_type _a in
   LowParse.Spec.BoundedInt.bounded_int32 min max
 
+let asn1_int32_min_of_type
+  (a: asn1_type)
+: asn1_int32
+= match a with
+  | BOOLEAN   -> 1ul
+  | NULL -> 0ul
+  | OCTET_STRING -> asn1_int32_min
+  | SEQUENCE -> asn1_int32_min
+
+let asn1_int32_max_of_type
+  (a: asn1_type)
+: asn1_int32
+= match a with
+  | BOOLEAN   -> 1ul
+  | NULL -> 0ul
+  | OCTET_STRING -> asn1_int32_max
+  | SEQUENCE -> asn1_int32_max
+
+let asn1_int32_bound_of_type
+  (a: asn1_type)
+: (asn1_int32 & asn1_int32)
+= (asn1_int32_min_of_type a, asn1_int32_max_of_type a)
+
+///
+let weak_kind_of_type
+  (a: asn1_type)
+: LowParse.Spec.Base.parser_kind
+= let min, max = asn1_length_bound_of_type a in
+  LowParse.Spec.Base.strong_parser_kind min max None
+
+///
 unfold
 let datatype_of_asn1_type (a: asn1_primitive_type): Type
 = match a with
   | BOOLEAN -> bool
-  // | INTEGER -> HI.pub_uint32
   | NULL -> unit
-  | OCTET_STRING -> (len: asn1_int32_of_tag OCTET_STRING & s: bytes {Seq.length s == v len})
+  | OCTET_STRING -> (len: asn1_int32_of_type OCTET_STRING & s: bytes {Seq.length s == v len})
 
 type asn1_value: Type =
 | BOOLEAN_VALUE: b: bool -> asn1_value
-| NULL_VALUE: n:unit -> asn1_value
-| OCTET_STRING_VALUE: len: asn1_int32_of_tag OCTET_STRING (* NOTE: Carrying length here for low-level operations. *)
+| NULL_VALUE: n: unit -> asn1_value
+| OCTET_STRING_VALUE: len: asn1_int32_of_type OCTET_STRING (* NOTE: Carrying length here for low-level operations. *)
                    -> s: bytes{v len == Seq.length s}
                    -> asn1_value
 
 unfold
-let asn1_value_of_tag (a: asn1_primitive_type): Type
+let asn1_value_of_type (a: asn1_primitive_type): Type
 = match a with
   | BOOLEAN      -> value: asn1_value{BOOLEAN_VALUE? value}
   | NULL         -> value: asn1_value{NULL_VALUE? value}
