src/asn1/ASN1.Low.NULL.fst
@@ -27,7 +27,7 @@ open ASN1.Low.Length
 
 let synth_asn1_null_TLV_inverse_impl
   (x: datatype_of_asn1_type NULL)
-: Tot (a: ((the_asn1_type NULL & asn1_int32_of_tag NULL) & datatype_of_asn1_type NULL){a == synth_asn1_null_TLV_inverse x})
+: Tot (a: ((the_asn1_type NULL & asn1_int32_of_type NULL) & datatype_of_asn1_type NULL){a == synth_asn1_null_TLV_inverse x})
 = ((NULL, len_of_asn1_data NULL x), x)
 
 let serialize32_asn1_null_TLV_backwards ()
@@ -35,7 +35,7 @@ let serialize32_asn1_null_TLV_backwards ()
 = serialize32_synth_backwards
    (* ls1*) (serialize32_the_asn1_tag_backwards NULL
              `serialize32_nondep_then_backwards`
-             serialize32_asn1_length_of_tag_backwards NULL
+             serialize32_asn1_length_of_type_backwards NULL
              `serialize32_nondep_then_backwards`
              serialize32_asn1_null_backwards ())
    (* f2 *) (synth_asn1_null_TLV)
