src/asn1/ASN1.Low.SEQUENCE.fst
@@ -1,0 +1,78 @@
+module ASN1.Low.SEQUENCE
+///
+/// ASN.1 Low
+///
+open LowParse.Low.Base
+open LowParse.Low.Combinators
+open LowParse.Low.FLData
+
+open ASN1.Base
+open ASN1.Spec.SEQUENCE
+open ASN1.Low.Base
+open ASN1.Low.Tag
+open ASN1.Low.Length
+
+module HS = FStar.HyperStack
+module HST = FStar.HyperStack.ST
+module B = LowStar.Buffer
+open FStar.Integers
+
+let serialize32_fldata_strong_backwards
+  (#k: parser_kind)
+  (#t: Type0)
+  (#p: parser k t)
+  (#s: serializer p)
+  (ls: serializer32_backwards s)
+  (len: asn1_int32)
+: Tot (serializer32_backwards (serialize_fldata_strong s (v len)))
+= fun (x: parse_fldata_strong_t s (v len))
+-> ls x
+
+let parser_tag_of_asn1_sequence_impl
+  (#k: parser_kind)
+  (#t: Type0)
+  (#p: parser k t)
+  (s: serializer p)
+  (len_of_data:
+    (data: t { asn1_length_inbound_of_type SEQUENCE (Seq.length (serialize s data)) })
+    -> Tot (len: asn1_int32_of_type SEQUENCE { v len == Seq.length (serialize s data) }))
+  (data: t { asn1_length_inbound_of_type SEQUENCE (Seq.length (serialize s data)) } )
+: Tot (tag: (the_asn1_type SEQUENCE & asn1_int32_of_type SEQUENCE) { tag == parser_tag_of_asn1_sequence s data })
+= (SEQUENCE, len_of_data data)
+
+let synth_asn1_sequence_value_inverse_impl
+  (#k: parser_kind)
+  (#t: Type0)
+  (#p: parser k t)
+  (s: serializer p)
+  (tag: (the_asn1_type SEQUENCE & asn1_int32_of_type SEQUENCE))
+  (data: refine_with_tag (parser_tag_of_asn1_sequence s) tag)
+: Tot (y: parse_fldata_strong_t s (v (snd tag)){ y == synth_asn1_sequence_value_inverse s tag data })
+= data <: refine_with_tag (parser_tag_of_asn1_sequence s) tag
+
+let serialize32_asn1_sequence_TLV_backwards
+  (#k: parser_kind)
+  (#t: Type0)
+  (#p: parser k t)
+  (#s: serializer p)
+  (ls: serializer32_backwards s)
+  (len_of_data:
+    (data: t { asn1_length_inbound_of_type SEQUENCE (Seq.length (serialize s data)) })
+    -> Tot (len: asn1_int32_of_type SEQUENCE { v len == Seq.length (serialize s data) }))
+: Tot (serializer32_backwards (serialize_asn1_sequence_TLV s))
+= serialize32_tagged_union_backwards
+  (* lst *) (serialize32_the_asn1_tag_backwards SEQUENCE
+             `serialize32_nondep_then_backwards`
+             serialize32_asn1_length_of_type_backwards SEQUENCE)
+  (* tag *) (parser_tag_of_asn1_sequence_impl s len_of_data)
+  (* s32 *) (fun (tag: the_asn1_type SEQUENCE & asn1_int32_of_type SEQUENCE)
+             -> let SEQUENCE, len = tag in
+                let l = v len in
+                (weak_kind_of_type SEQUENCE
+                 `serialize32_weaken_backwards`
+                (serialize32_synth_backwards
+                 (* ls1 *) (serialize32_fldata_strong_backwards ls len)
+                 (* f2  *) (synth_asn1_sequence_value s tag)
+                 (* g1  *) (synth_asn1_sequence_value_inverse s tag)
+                 (* g1' *) (synth_asn1_sequence_value_inverse_impl s tag)
+                 (* prf *) ())) <: serializer32_backwards (serialize_asn1_sequence_value_weak s tag))
