src/asn1/ASN1.Spec.OCTET_STRING.fst
@@ -62,23 +62,23 @@ let serialize_asn1_octet_string_weak
 /// Specialized TLV
 ///
 // let synth_asn1_octet_string_L
-//   (x: the_asn1_type OCTET_STRING & asn1_len_of_tag OCTET_STRING)
-// : GTot (asn1_len_of_tag OCTET_STRING)
+//   (x: the_asn1_type OCTET_STRING & asn1_len_of_type OCTET_STRING)
+// : GTot (asn1_len_of_type OCTET_STRING)
 // = snd x
 
 // let synth_asn1_octet_string_L_inverse
-//   (len: asn1_len_of_tag OCTET_STRING)
-// : GTot (x: (the_asn1_type OCTET_STRING & asn1_len_of_tag OCTET_STRING){len == synth_asn1_octet_string_L x})
+//   (len: asn1_len_of_type OCTET_STRING)
+// : GTot (x: (the_asn1_type OCTET_STRING & asn1_len_of_type OCTET_STRING){len == synth_asn1_octet_string_L x})
 // = (OCTET_STRING, len)
 
 let parser_tag_of_octet_string
   (x: datatype_of_asn1_type OCTET_STRING)
-: GTot (the_asn1_type OCTET_STRING & asn1_int32_of_tag OCTET_STRING)
+: GTot (the_asn1_type OCTET_STRING & asn1_int32_of_type OCTET_STRING)
 = (OCTET_STRING, dfst x)
 
 let synth_asn1_octet_string_data
-  (len: asn1_int32_of_tag OCTET_STRING)
-  (x: the_asn1_type OCTET_STRING & asn1_int32_of_tag OCTET_STRING{x == (OCTET_STRING, len)})
+  (len: asn1_int32_of_type OCTET_STRING)
+  (x: the_asn1_type OCTET_STRING & asn1_int32_of_type OCTET_STRING{x == (OCTET_STRING, len)})
   (s: lbytes (v len))
 : GTot (refine_with_tag parser_tag_of_octet_string x)
 = let value: datatype_of_asn1_type OCTET_STRING = (|len, s|) in
@@ -86,22 +86,22 @@ let synth_asn1_octet_string_data
   y
 
 let synth_asn1_octet_string_data_inverse
-  (len: asn1_int32_of_tag OCTET_STRING)
-  (x: the_asn1_type OCTET_STRING & asn1_int32_of_tag OCTET_STRING{x == (OCTET_STRING, len)})
+  (len: asn1_int32_of_type OCTET_STRING)
+  (x: the_asn1_type OCTET_STRING & asn1_int32_of_type OCTET_STRING{x == (OCTET_STRING, len)})
   (value: refine_with_tag parser_tag_of_octet_string x)
 : GTot (s: lbytes (v len))
 = dsnd
-    #(asn1_int32_of_tag OCTET_STRING)
-    #(fun (len:asn1_int32_of_tag OCTET_STRING) -> s:bytes{Seq.length s == v len})
+    #(asn1_int32_of_type OCTET_STRING)
+    #(fun (len:asn1_int32_of_type OCTET_STRING) -> s:bytes{Seq.length s == v len})
     value
 
 let parse_asn1_octet_string_kind_strong
-  (x: the_asn1_type OCTET_STRING & asn1_int32_of_tag OCTET_STRING)
+  (x: the_asn1_type OCTET_STRING & asn1_int32_of_type OCTET_STRING)
 : parser_kind
 = total_constant_size_parser_kind (v (snd x))
 
 let parse_asn1_octet_string_data
-  (x: the_asn1_type OCTET_STRING & asn1_int32_of_tag OCTET_STRING)
+  (x: the_asn1_type OCTET_STRING & asn1_int32_of_type OCTET_STRING)
 : Tot (parser (parse_asn1_octet_string_kind_strong x) (refine_with_tag parser_tag_of_octet_string x))
 = parse_asn1_octet_string (v (snd x))
   `parse_synth`
@@ -110,11 +110,11 @@ let parse_asn1_octet_string_data
 let parse_asn1_octet_string_data_unfold
   (input: bytes)
 : Lemma (
-  forall (x: the_asn1_type OCTET_STRING & asn1_int32_of_tag OCTET_STRING).
+  forall (x: the_asn1_type OCTET_STRING & asn1_int32_of_type OCTET_STRING).
 )
 
 let serialize_asn1_octet_string_data
-  (x: the_asn1_type OCTET_STRING & asn1_int32_of_tag OCTET_STRING)
+  (x: the_asn1_type OCTET_STRING & asn1_int32_of_type OCTET_STRING)
 : Tot (serializer (parse_asn1_octet_string_data x))
 = serialize_synth
   (* p1 *) (parse_asn1_octet_string (v (snd x)))
@@ -124,14 +124,14 @@ let serialize_asn1_octet_string_data
   (* Prf*) ()
 
 let parse_asn1_octet_string_data_weak
-  (x: the_asn1_type OCTET_STRING & asn1_int32_of_tag OCTET_STRING)
+  (x: the_asn1_type OCTET_STRING & asn1_int32_of_type OCTET_STRING)
 : Tot (parser parse_asn1_octet_string_kind_weak (refine_with_tag parser_tag_of_octet_string x))
 = parse_asn1_octet_string_kind_weak
   `weaken`
   parse_asn1_octet_string_data x
 
 let serialize_asn1_octet_string_data_weak
-  (x: the_asn1_type OCTET_STRING & asn1_int32_of_tag OCTET_STRING)
+  (x: the_asn1_type OCTET_STRING & asn1_int32_of_type OCTET_STRING)
 : Tot (serializer (parse_asn1_octet_string_data_weak x))
 = parse_asn1_octet_string_kind_weak
   `serialize_weaken`
@@ -148,7 +148,7 @@ let parse_asn1_octet_string_TLV_kind
 : parser_kind
 = parse_asn1_tag_kind
   `and_then_kind`
-  parse_asn1_length_kind_of_tag OCTET_STRING
+  parse_asn1_length_kind_of_type OCTET_STRING
   `and_then_kind`
   parse_asn1_octet_string_kind_weak
 
@@ -157,7 +157,7 @@ let parse_asn1_octet_string_TLV
 = parse_tagged_union
   (* pt *) (parse_the_asn1_tag OCTET_STRING
             `nondep_then`
-            parse_asn1_length_of_tag OCTET_STRING)
+            parse_asn1_length_of_type OCTET_STRING)
   (* tg *) (parser_tag_of_octet_string)
   (* p  *) (parse_asn1_octet_string_data_weak)
 
@@ -169,7 +169,7 @@ let parse_asn1_octet_string_TLV_unfold
   | None -> None
   | Some (v_T, l_T) ->
     (let input_LV = Seq.slice input l_T (Seq.length input) in
-     match parse (parse_asn1_length_of_tag OCTET_STRING) input_LV with
+     match parse (parse_asn1_length_of_type OCTET_STRING) input_LV with
      | None -> None
      | Some (v_L, l_L) ->
        (let input_data = Seq.slice input_LV l_L (Seq.length input_LV) in
@@ -180,7 +180,7 @@ let parse_asn1_octet_string_TLV_unfold
 )
 = nondep_then_eq
   (* p1 *) (parse_the_asn1_tag OCTET_STRING)
-  (* p2 *) (parse_asn1_length_of_tag OCTET_STRING)
+  (* p2 *) (parse_asn1_length_of_type OCTET_STRING)
   (* in *) (input);
   parse_synth_eq
   (* p1 *) (parse_asn1_octet_string (v (snd x)))
@@ -192,7 +192,7 @@ let serialize_asn1_octet_string_TLV
 = serialize_tagged_union
   (* st *) (serialize_the_asn1_tag OCTET_STRING
             `serialize_nondep_then`
-            serialize_asn1_length_of_tag OCTET_STRING)
+            serialize_asn1_length_of_type OCTET_STRING)
   (* tg *) (parser_tag_of_octet_string)
   (* s  *) (serialize_asn1_octet_string_data_weak)
 
@@ -203,5 +203,5 @@ let length_lemma
   (ensures (
     let px = parse parse_asn1_octet_string_TLV input in
     let pt = parse (parse_the_asn1_tag OCTET_STRING) input in
-    let pl = parse (parse_asn1_length_of_tag OCTET_STRING) (Seq.slice input 0 )
+    let pl = parse (parse_asn1_length_of_type OCTET_STRING) (Seq.slice input 0 )
   ))
