src/asn1/ASN1.Spec.SEQUENCE.fst
@@ -1,0 +1,141 @@
+module ASN1.Spec.SEQUENCE
+
+open ASN1.Base
+open ASN1.Spec.Tag
+open ASN1.Spec.Length
+open LowParse.Bytes
+open LowParse.Spec.FLData
+
+open FStar.Integers
+
+/// ASN.1 SEQUENCE Tag-Length parser/serializer
+///
+///
+let parse_asn1_sequence_TL_kind
+: parser_kind
+= parse_asn1_tag_kind
+  `and_then_kind`
+  parse_asn1_length_kind_of_type SEQUENCE
+
+let parse_asn1_sequence_TL
+: parser parse_asn1_sequence_TL_kind (the_asn1_type SEQUENCE & asn1_int32_of_type SEQUENCE)
+= parse_the_asn1_tag SEQUENCE
+  `nondep_then`
+  parse_asn1_length_of_type SEQUENCE
+
+let serialize_asn1_sequence_TL
+: serializer parse_asn1_sequence_TL
+= serialize_the_asn1_tag SEQUENCE
+  `serialize_nondep_then`
+  serialize_asn1_length
+
+/// Tagging function
+///
+///
+let parser_tag_of_asn1_sequence
+  (#k: parser_kind)
+  (#t: Type0)
+  (#p: parser k t)
+  (s: serializer p)
+  (data: t { asn1_length_inbound_of_type SEQUENCE (Seq.length (serialize s data)) } )
+: GTot (the_asn1_type SEQUENCE & asn1_int32_of_type SEQUENCE)
+= (SEQUENCE, u (Seq.length (serialize s data)))
+
+let synth_asn1_sequence_value
+  (#k: parser_kind)
+  (#t: Type0)
+  (#p: parser k t)
+  (s: serializer p)
+  (tag: (the_asn1_type SEQUENCE & asn1_int32_of_type SEQUENCE))
+  (y: parse_fldata_strong_t s (v (snd tag)))
+: GTot (data: refine_with_tag (parser_tag_of_asn1_sequence s) tag)
+= y <: refine_with_tag (parser_tag_of_asn1_sequence s) tag
+
+let synth_asn1_sequence_value_inverse
+  (#k: parser_kind)
+  (#t: Type0)
+  (#p: parser k t)
+  (s: serializer p)
+  (tag: (the_asn1_type SEQUENCE & asn1_int32_of_type SEQUENCE))
+  (data: refine_with_tag (parser_tag_of_asn1_sequence s) tag)
+: GTot (y: parse_fldata_strong_t s (v (snd tag)){ data == synth_asn1_sequence_value s tag y })
+= data <: refine_with_tag (parser_tag_of_asn1_sequence s) tag
+
+/// ASN.1 SEQUENCE value parser/serializer
+///
+///
+let parse_asn1_sequence_value
+  (#k: parser_kind)
+  (#t: Type0)
+  (#p: parser k t)
+  (s: serializer p)
+  (tag: the_asn1_type SEQUENCE & asn1_int32_of_type SEQUENCE)
+: parser (parse_fldata_kind (v (snd tag)) k) (refine_with_tag (parser_tag_of_asn1_sequence s) tag)
+= serializer_correct_implies_complete p s;
+  parse_fldata_strong s (v (snd tag))
+  `parse_synth`
+  synth_asn1_sequence_value s tag
+
+let parse_asn1_sequence_value_weak
+  (#k: parser_kind)
+  (#t: Type0)
+  (#p: parser k t)
+  (s: serializer p)
+  (tag: the_asn1_type SEQUENCE & asn1_int32_of_type SEQUENCE)
+: parser (weak_kind_of_type SEQUENCE) (refine_with_tag (parser_tag_of_asn1_sequence s) tag)
+= weak_kind_of_type SEQUENCE
+  `weaken`
+  parse_asn1_sequence_value s tag
+
+let serialize_asn1_sequence_value
+  (#k: parser_kind)
+  (#t: Type0)
+  (#p: parser k t)
+  (s: serializer p)
+  (tag: the_asn1_type SEQUENCE & asn1_int32_of_type SEQUENCE)
+: serializer (parse_asn1_sequence_value s tag)
+= serializer_correct_implies_complete p s;
+  serialize_synth
+  (* p1 *) (parse_fldata_strong s (v (snd tag)))
+  (* f2 *) (synth_asn1_sequence_value s tag)
+  (* s1 *) (serialize_fldata_strong s (v (snd tag)))
+  (* g1 *) (synth_asn1_sequence_value_inverse s tag)
+  (* prf*) ()
+
+let serialize_asn1_sequence_value_weak
+  (#k: parser_kind)
+  (#t: Type0)
+  (#p: parser k t)
+  (s: serializer p)
+  (tag: the_asn1_type SEQUENCE & asn1_int32_of_type SEQUENCE)
+: serializer (parse_asn1_sequence_value_weak s tag)
+= weak_kind_of_type SEQUENCE
+  `serialize_weaken`
+  serialize_asn1_sequence_value s tag
+
+/// Specialized TLV parser/serializer
+///
+///
+
+let parse_asn1_sequence_TLV
+  (#k: parser_kind)
+  (#t: Type0)
+  (#p: parser k t)
+  (s: serializer p)
+= parse_tagged_union
+  (* pt *) (parse_asn1_sequence_TL)
+  (* tg *) (parser_tag_of_asn1_sequence s)
+  (* p  *) (parse_asn1_sequence_value_weak s)
+
+let serialize_asn1_sequence_TLV
+  (#k: parser_kind)
+  (#t: Type0)
+  (#p: parser k t)
+  (s: serializer p)
+: Tot (serializer (parse_asn1_sequence_TLV s))
+= serialize_tagged_union
+  (* st *) (serialize_asn1_sequence_TL)
+  (* tg *) (parser_tag_of_asn1_sequence s)
+  (* s  *) (serialize_asn1_sequence_value_weak s)
+
+
